Interface.v
@@ -5,6 +5,7 @@ Require Import Rustre.Common.
 Require compcert.common.Values.
 Require compcert.cfrontend.Cop.
 Require compcert.cfrontend.Ctypes.
+Require compcert.cfrontend.Ctyping.
 Require compcert.common.Memory.
 Require compcert.lib.Maps.
 
@@ -15,16 +16,37 @@ Definition empty_composite_env : Ctypes.composite_env := (Maps.PTree.empty _).
 Module Export Op <: OPERATORS.
   Definition val: Type := Values.val.
 
-  (* TODO: wrong! Fix. *)
-  Definition typ := Ctypes.type.
+  Inductive type' : Type :=
+  | Tbool:  type'
+  | Tint:   Ctypes.intsize -> Ctypes.signedness -> type'
+  | Tlong:  Ctypes.signedness -> type'
+  | Tfloat: Ctypes.floatsize -> type'.
 
+  Definition type := type'.
+
+  Definition cltype (ty: type) : Ctypes.type :=
+    match ty with
+    | Tbool      => Ctypes.type_bool
+    | Tint sz sg => Ctypes.Tint sz sg Ctypes.noattr
+    | Tlong sg   => Ctypes.Tlong sg Ctypes.noattr
+    | Tfloat sz  => Ctypes.Tfloat sz Ctypes.noattr
+    end.
+
+  Definition typecl (ty: Ctypes.type) : option type :=
+    match ty with
+    | Ctypes.Tint sz sg (Ctypes.mk_attr false None) => Some (Tint sz sg)
+    | Ctypes.Tlong sg   (Ctypes.mk_attr false None) => Some (Tlong sg)
+    | Ctypes.Tfloat sz  (Ctypes.mk_attr false None) => Some (Tfloat sz)
+    | _ => None
+    end.
+  
   Definition true_val := Values.Vtrue.
   Definition false_val := Values.Vfalse.
 
   Lemma true_not_false_val: true_val <> false_val.
   Proof. discriminate. Qed.
 
-  Definition bool_typ := Ctypes.type_bool.
+  Definition bool_type : type := Tbool.
 
   Inductive constant : Type :=
   | Cint: Integers.int -> Ctypes.intsize -> Ctypes.signedness -> constant
@@ -34,12 +56,12 @@ Module Export Op <: OPERATORS.
 
   Definition const := constant.
 
-  Definition typ_const (c: const) : typ :=
+  Definition type_const (c: const) : type :=
     match c with
-    | Cint _ sz sg => Ctypes.Tint sz sg Ctypes.noattr
-    | Clong _ sg   => Ctypes.Tlong sg Ctypes.noattr
-    | Cfloat _     => Ctypes.Tfloat Ctypes.F64 Ctypes.noattr
-    | Csingle _    => Ctypes.Tfloat Ctypes.F32 Ctypes.noattr
+    | Cint _ sz sg => Tint sz sg
+    | Clong _ sg   => Tlong sg
+    | Cfloat _     => Tfloat Ctypes.F64
+    | Csingle _    => Tfloat Ctypes.F32
     end.
 
   Definition sem_const (c: const) : val :=
@@ -50,38 +72,69 @@ Module Export Op <: OPERATORS.
     | Csingle f  => Values.Vsingle f
     end.
 
-  Definition unary_op := Cop.unary_operation.
+  Inductive unary_op' : Type :=
+  | UnaryOp: Cop.unary_operation -> unary_op'
+  | CastOp:  type -> unary_op'.
+
+  Definition unary_op := unary_op'.
   Definition binary_op := Cop.binary_operation.
 
-  Definition sem_unary (op: unary_op) (v: val) (ty: typ) : option val :=
-    Cop.sem_unary_operation op v ty Memory.Mem.empty.
+  Definition sem_unary (uop: unary_op) (v: val) (ty: type) : option val :=
+    match uop with
+    | UnaryOp op => Cop.sem_unary_operation op v (cltype ty) Memory.Mem.empty
+    | CastOp ty' => Cop.sem_cast v (cltype ty) (cltype ty') Memory.Mem.empty
+    end.
 
   Definition sem_binary (op: binary_op)
-             (v1: val) (ty1: typ)
-             (v2: val) (ty2: typ) : option val :=
+             (v1: val) (ty1: type)
+             (v2: val) (ty2: type) : option val :=
     Cop.sem_binary_operation
-      empty_composite_env op v1 ty1 v2 ty2 Memory.Mem.empty.
+      empty_composite_env op v1 (cltype ty1) v2 (cltype ty2) Memory.Mem.empty.
+
+  Definition type_unary (uop: unary_op) (ty: type) : option type :=
+    match uop with
+    | UnaryOp op => match Ctyping.type_unop op (cltype ty) with
+                    | Errors.OK ty' => typecl ty'
+                    | Errors.Error _ => None
+                    end
+    | CastOp ty' => match Ctyping.check_cast (cltype ty) (cltype ty') with
+                    | Errors.OK _ => Some ty'
+                    | Errors.Error _ => None
+                    end
+    end.
+
+  Definition type_binary (op: binary_op) (ty1 ty2: type) : option type :=
+    match Ctyping.type_binop op (cltype ty1) (cltype ty2) with
+    | Errors.OK ty' => typecl ty'
+    | Errors.Error _ => None
+    end.
 
   Lemma val_dec   : forall v1 v2 : val, {v1 = v2} + {v1 <> v2}.
   Proof Values.Val.eq.
 
-  Lemma typ_dec   : forall t1 t2 : typ, {t1 = t2} + {t1 <> t2}.
-  Proof Ctypes.type_eq.
+  Lemma type_dec   : forall t1 t2 : type, {t1 = t2} + {t1 <> t2}.
+  Proof.
+    decide equality; (apply Ctyping.signedness_eq
+                      || apply Ctyping.intsize_eq
+                      || apply Ctyping.floatsize_eq).
+  Qed.
   
   Lemma const_dec : forall c1 c2 : const, {c1 = c2} + {c1 <> c2}.
   Proof.
-    assert (forall (x y: Ctypes.intsize), {x=y} + {x<>y}) by decide equality.
-    assert (forall (x y: Ctypes.signedness), {x=y} + {x<>y}) by decide equality.
-    decide equality.
-    apply Int.eq_dec.
-    apply Int64.eq_dec.
-    apply Float.eq_dec.
-    apply Float32.eq_dec.
+    decide equality; (apply Ctyping.signedness_eq
+                      || apply Ctyping.intsize_eq
+                      || apply Int.eq_dec
+                      || apply Int64.eq_dec
+                      || apply Float.eq_dec
+                      || apply Float32.eq_dec).
   Qed.
-      
+
   Lemma unop_dec  : forall op1 op2 : unary_op, {op1 = op2} + {op1 <> op2}.
   Proof.
+    assert (forall (x y: Cop.unary_operation), {x=y} + {x<>y})
+      by decide equality.
     decide equality.
+    apply type_dec.
   Qed.
 
   Lemma binop_dec : forall op1 op2 : binary_op, {op1 = op2} + {op1 <> op2}.
@@ -90,3 +143,4 @@ Module Export Op <: OPERATORS.
   Qed.
     
 End Op.
+
